isabelle: Extend parser to cover modules, statements, etc. (WIP)

isabelle/BabParser.thy
@@ -1,5 +1,5 @@
 theory BabParser
-  imports Main Location BabSyntax BasicParser
+  imports Main "HOL-Library.Char_ord" Location BabSyntax BasicParser
 begin
 
 (* Specializing BasicParser for our parser *)
@@ -95,10 +95,29 @@ definition parse_dotted_name :: "string Parser" where
 
 (* TYPE AND TERM PARSING *)
 
+(* Type parsing helpers: *)
+
 (* helper to make an array type *)
 fun make_array_type :: "(Location \<times> BabDimension list) \<Rightarrow> BabType \<Rightarrow> BabType" where
   "make_array_type (loc, dims) ty =
     BabTy_Array (merge_locations (bab_type_location ty) loc) ty dims"
+
+(* Parse a type that can be used in a numeric cast expression (like `i8(x)`) *)
+definition parse_numeric_type :: "BabType Parser" where
+  "parse_numeric_type = with_loc (
+    (expect (KEYWORD KW_I8) \<then> return (\<lambda>loc. BabTy_FiniteInt loc Signed IntBits_8))
+    <|> (expect (KEYWORD KW_I16) \<then> return (\<lambda>loc. BabTy_FiniteInt loc Signed IntBits_16))
+    <|> (expect (KEYWORD KW_I32) \<then> return (\<lambda>loc. BabTy_FiniteInt loc Signed IntBits_32))
+    <|> (expect (KEYWORD KW_I64) \<then> return (\<lambda>loc. BabTy_FiniteInt loc Signed IntBits_64))
+    <|> (expect (KEYWORD KW_U8) \<then> return (\<lambda>loc. BabTy_FiniteInt loc Unsigned IntBits_8))
+    <|> (expect (KEYWORD KW_U16) \<then> return (\<lambda>loc. BabTy_FiniteInt loc Unsigned IntBits_16))
+    <|> (expect (KEYWORD KW_U32) \<then> return (\<lambda>loc. BabTy_FiniteInt loc Unsigned IntBits_32))
+    <|> (expect (KEYWORD KW_U64) \<then> return (\<lambda>loc. BabTy_FiniteInt loc Unsigned IntBits_64))
+    <|> (expect (KEYWORD KW_INT) \<then> return BabTy_MathInt)
+    <|> (expect (KEYWORD KW_REAL) \<then> return BabTy_MathReal))"
+
+
+(* Term parsing helpers: *)
 
 (* Parse an int literal token *)
 definition int_literal :: "BabLiteral Parser" where
@@ -114,7 +133,7 @@ definition string_literal :: "BabLiteral Parser" where
     case t of STRING s \<Rightarrow> return (BabLit_String s)
   }"
 
-(* Binop parsing *)
+(* Parse a binop token *)
 (* If successful, returns a precedence and the corresponding binop *)
 definition parse_binop :: "(nat \<times> BabBinop) Parser" where
   "parse_binop = 
@@ -146,7 +165,7 @@ definition parse_binop :: "(nat \<times> BabBinop) Parser" where
 
   <|> (expect LESS_EQUAL_EQUAL_GREATER \<then> return (1, BabBinop_Iff))"
 
-(* parse a binop of at least the given precedence *)
+(* Parse a binop token of at least the given precedence *)
 fun binop_of_at_least_prec :: "nat \<Rightarrow> (nat \<times> BabBinop) Parser" where
   "binop_of_at_least_prec min_prec = do {
     p \<leftarrow> parse_binop;
@@ -155,11 +174,6 @@ fun binop_of_at_least_prec :: "nat \<Rightarrow> (nat \<times> BabBinop) Parser"
     else
       fail)
     }"
-
-(* helper to make a binop term *)
-fun make_binop_term :: "BabTerm \<Rightarrow> BabBinop \<times> BabTerm \<Rightarrow> BabTerm" where
-  "make_binop_term lhs (op, rhs) =
-    BabTm_Binop (merge_locations (bab_term_location lhs) (bab_term_location rhs)) op lhs rhs"
 
 (* unary operators *)
 fun unary_operator :: "Token \<Rightarrow> BabUnop option" where
@@ -183,19 +197,27 @@ fun make_unop_term :: "Location \<times> BabUnop \<Rightarrow> BabTerm \<Rightar
 | "make_unop_term (loc, op) tm
     = BabTm_Unop (merge_locations loc (bab_term_location tm)) op tm"
 
+(* Note: a "restricted" term is one that cannot contain the curly-brace function
+   call syntax (e.g. `f{1,2,3}`). This is used to avoid ambiguities in certain
+   contexts e.g. if-conditions. It is our equivalent of the following Rust issue:
+   https://github.com/rust-lang/rust/issues/50090. *)
+datatype Restrict = Restricted | Unrestricted
+
+
 (* Mutually recursive type and term parsing functions *)
+
 fun parse_type_fuelled :: "nat \<Rightarrow> BabType Parser"
   and parse_basic_type :: "nat \<Rightarrow> BabType Parser"
   and parse_optional_tyargs :: "nat \<Rightarrow> BabType list Parser"
   and parse_name_type_pair :: "nat \<Rightarrow> (string \<times> BabType) Parser"
   and parse_array_suffix :: "nat \<Rightarrow> BabDimension list Parser"
   and parse_array_dimension :: "nat \<Rightarrow> BabDimension Parser"
-  and parse_term_min :: "nat \<Rightarrow> nat \<Rightarrow> BabTerm Parser"
-  and parse_operator_and_term :: "nat \<Rightarrow> nat \<Rightarrow> (BabBinop \<times> BabTerm) Parser"
-  and parse_unop_expr :: "nat \<Rightarrow> BabTerm Parser"
-  and parse_call_or_proj_expr :: "nat \<Rightarrow> BabTerm Parser"
-  and parse_call_or_proj_suffix :: "nat \<Rightarrow> (BabTerm \<Rightarrow> BabTerm) Parser"
-  and parse_primary_expr :: "nat \<Rightarrow> BabTerm Parser"
+  and parse_term_min :: "nat \<Rightarrow> nat \<Rightarrow> Restrict \<Rightarrow> BabTerm Parser"
+  and parse_operator_and_term :: "nat \<Rightarrow> nat \<Rightarrow> Restrict \<Rightarrow> (BabBinop \<times> BabTerm) Parser"
+  and parse_unop_expr :: "nat \<Rightarrow> Restrict \<Rightarrow> BabTerm Parser"
+  and parse_call_or_proj_expr :: "nat \<Rightarrow> Restrict \<Rightarrow> BabTerm Parser"
+  and parse_call_or_proj_suffix :: "nat \<Rightarrow> Restrict \<Rightarrow> (BabTerm \<Rightarrow> BabTerm) Parser"
+  and parse_primary_expr :: "nat \<Rightarrow> Restrict \<Rightarrow> BabTerm Parser"
 where
 
 (* Parse a type *)
@@ -213,23 +235,14 @@ where
    field projection (i.e. there is no ambiguity with dots) *)
 | "parse_basic_type fuel =
   (parens (delay (\<lambda>_. parse_type_fuelled fuel)))
-  <|> with_loc (     
+  <|> parse_numeric_type
+  <|> with_loc (
         (expect (KEYWORD KW_BOOL) \<then> return BabTy_Bool)
     <|> (do {
           name \<leftarrow> parse_dotted_name;
           args \<leftarrow> parse_optional_tyargs fuel;
           return (\<lambda>loc. BabTy_Name loc name args)
         })
-    <|> (expect (KEYWORD KW_I8) \<then> return (\<lambda>loc. BabTy_FiniteInt loc Signed IntBits_8))
-    <|> (expect (KEYWORD KW_I16) \<then> return (\<lambda>loc. BabTy_FiniteInt loc Signed IntBits_16))
-    <|> (expect (KEYWORD KW_I32) \<then> return (\<lambda>loc. BabTy_FiniteInt loc Signed IntBits_32))
-    <|> (expect (KEYWORD KW_I64) \<then> return (\<lambda>loc. BabTy_FiniteInt loc Signed IntBits_64))
-    <|> (expect (KEYWORD KW_U8) \<then> return (\<lambda>loc. BabTy_FiniteInt loc Unsigned IntBits_8))
-    <|> (expect (KEYWORD KW_U16) \<then> return (\<lambda>loc. BabTy_FiniteInt loc Unsigned IntBits_16))
-    <|> (expect (KEYWORD KW_U32) \<then> return (\<lambda>loc. BabTy_FiniteInt loc Unsigned IntBits_32))
-    <|> (expect (KEYWORD KW_U64) \<then> return (\<lambda>loc. BabTy_FiniteInt loc Unsigned IntBits_64))
-    <|> (expect (KEYWORD KW_INT) \<then> return BabTy_MathInt)
-    <|> (expect (KEYWORD KW_REAL) \<then> return BabTy_MathReal)
     <|> (do {
           fieldTypes \<leftarrow> braces (comma_list (delay (\<lambda>_. parse_type_fuelled fuel)));
           return (\<lambda>loc. BabTy_Tuple loc fieldTypes)
@@ -253,6 +266,7 @@ where
     return (name, ty)
    }"
 
+
 (* Parse an array-dimension-list in brackets *)
 | "parse_array_suffix fuel = 
     brackets (comma_list (parse_array_dimension fuel))"
@@ -260,53 +274,55 @@ where
 (* Parse a single array dimension *)
 | "parse_array_dimension fuel =
     (expect STAR \<then> return BabDim_Allocatable)
-    <|> (delay (\<lambda>_. parse_term_min fuel 0) \<bind> (return \<circ> BabDim_Fixed))
+    <|> (delay (\<lambda>_. parse_term_min fuel 0 Unrestricted) \<bind> (return \<circ> BabDim_Fixed))
     <|> (return BabDim_Unknown)"
 
 (* Parse a term, followed by zero or more operator-term pairs at given precedence or higher *)
-| "parse_term_min 0 _ = undefined"   (* out of fuel *)
-| "parse_term_min (Suc fuel) min_prec = do {
-    left \<leftarrow> parse_unop_expr fuel;
-    others \<leftarrow> many (parse_operator_and_term fuel min_prec);
-    return (foldl make_binop_term left others)
-  }"
+| "parse_term_min 0 _ _ = undefined"   (* out of fuel *)
+| "parse_term_min (Suc fuel) min_prec restrict = with_loc (do {
+    left \<leftarrow> parse_unop_expr fuel restrict;
+    others \<leftarrow> many (parse_operator_and_term fuel min_prec restrict);
+    return (\<lambda>loc. BabTm_Binop loc left others)
+  })"
 
 (* Parse operator-term pair at given precedence or higher *)
-| "parse_operator_and_term fuel min_prec =
+| "parse_operator_and_term fuel min_prec restrict =
     do {
       p \<leftarrow> binop_of_at_least_prec min_prec;
-      term \<leftarrow> parse_term_min fuel (Suc (fst p));
+      term \<leftarrow> parse_term_min fuel (Suc (fst p)) restrict;
       return (snd p, term)
     }"
 
 (* Parse unary operator expression *)
-| "parse_unop_expr fuel = do {
+| "parse_unop_expr fuel restrict = do {
     ops \<leftarrow> many (located parse_unop);
-    tm \<leftarrow> parse_call_or_proj_expr fuel;
+    tm \<leftarrow> parse_call_or_proj_expr fuel restrict;
     return (foldr make_unop_term ops tm)
   }"
 
 (* Parse function call, field projection or array projection *)
-| "parse_call_or_proj_expr fuel = do {
-    tm \<leftarrow> parse_primary_expr fuel;
-    suffixes \<leftarrow> many (parse_call_or_proj_suffix fuel);
+| "parse_call_or_proj_expr fuel restrict = do {
+    tm \<leftarrow> parse_primary_expr fuel restrict;
+    suffixes \<leftarrow> many (parse_call_or_proj_suffix fuel restrict);
     return (foldl (\<lambda>tm f. f tm) tm suffixes)
   }"
 
-| "parse_call_or_proj_suffix fuel =
+| "parse_call_or_proj_suffix fuel restrict =
     (do {
-      loc_and_args \<leftarrow> located (parens (comma_list (delay (\<lambda>_. parse_term_min fuel 0))));
+      loc_and_args \<leftarrow> located (parens (comma_list (delay (\<lambda>_. parse_term_min fuel 0 Unrestricted))));
       return (\<lambda>tm. BabTm_Call (merge_locations (bab_term_location tm) (fst loc_and_args))
                               tm
                               (snd loc_and_args))
     })
-  <|> (do {
-        look_ahead (expect LBRACE);
-        loc_and_arg \<leftarrow> located (delay (\<lambda>_. parse_primary_expr fuel));
-        return (\<lambda>tm. BabTm_Call (merge_locations (bab_term_location tm) (fst loc_and_arg))
-                                tm
-                                [snd loc_and_arg])
-      })
+  <|> (if restrict = Unrestricted then
+        (do {
+          look_ahead (expect LBRACE);
+          loc_and_arg \<leftarrow> located (delay (\<lambda>_. parse_primary_expr fuel Unrestricted));
+          return (\<lambda>tm. BabTm_Call (merge_locations (bab_term_location tm) (fst loc_and_arg))
+                                  tm
+                                  [snd loc_and_arg])
+        })
+       else fail)
   <|> (do {
         expect DOT;
         loc_and_fld \<leftarrow> located (satisfy is_nat_num_token);
@@ -326,16 +342,15 @@ where
                                           n))
       })
   <|> (do {
-        loc_and_idxs \<leftarrow> located (brackets (comma_list (delay (\<lambda>_. parse_term_min fuel 0))));
+        loc_and_idxs \<leftarrow> located (brackets (comma_list (delay (\<lambda>_. parse_term_min fuel 0 Unrestricted))));
         return (\<lambda>tm. BabTm_ArrayProj (merge_locations (bab_term_location tm) (fst loc_and_idxs))
                                      tm
                                      (snd loc_and_idxs))
       })"
 
 (* Parse a primary expression, e.g. variable name, literal, parenthesized expression *)
-(* TODO: Finish this - add more cases *)
-| "parse_primary_expr fuel =
-    (parens (delay (\<lambda>_. parse_term_min fuel 0)))
+| "parse_primary_expr fuel restrict =
+    (parens (delay (\<lambda>_. parse_term_min fuel 0 Unrestricted)))
   <|> with_loc (
         (int_literal \<bind> (\<lambda>lit. return (\<lambda>loc. BabTm_Literal loc lit)))
     <|> (string_literal \<bind> (\<lambda>lit. return (\<lambda>loc. BabTm_Literal loc lit)))
@@ -348,28 +363,82 @@ where
         })
     <|> (do {
           expect (KEYWORD KW_IF);
-          tm1 \<leftarrow> delay (\<lambda>_. parse_term_min fuel 0);
+          tm1 \<leftarrow> delay (\<lambda>_. parse_term_min fuel 0 Unrestricted);
           expect (KEYWORD KW_THEN);
-          tm2 \<leftarrow> delay (\<lambda>_. parse_term_min fuel 0);
+          tm2 \<leftarrow> delay (\<lambda>_. parse_term_min fuel 0 Unrestricted);
           expect (KEYWORD KW_ELSE);
-          tm3 \<leftarrow> delay (\<lambda>_. parse_term_min fuel 0);
+          tm3 \<leftarrow> delay (\<lambda>_. parse_term_min fuel 0 restrict);
           return (\<lambda>loc. BabTm_If loc tm1 tm2 tm3)
         })
     <|> (do {
           expect (KEYWORD KW_LET);
           name \<leftarrow> parse_name;
           expect EQUAL;
-          tm1 \<leftarrow> delay (\<lambda>_. parse_term_min fuel 0);
+          tm1 \<leftarrow> delay (\<lambda>_. parse_term_min fuel 0 Unrestricted);
           expect (KEYWORD KW_IN);
-          tm2 \<leftarrow> delay (\<lambda>_. parse_term_min fuel 0);
+          tm2 \<leftarrow> delay (\<lambda>_. parse_term_min fuel 0 restrict);
           return (\<lambda>loc. BabTm_Let loc name tm1 tm2)
         })
     <|> (do {
           quant \<leftarrow> (expect (KEYWORD KW_FORALL) <|> expect (KEYWORD KW_EXISTS));
           name_ty \<leftarrow> parens (parse_name_type_pair fuel);
-          tm \<leftarrow> delay (\<lambda>_. parse_term_min fuel 0);
+          tm \<leftarrow> delay (\<lambda>_. parse_term_min fuel 0 Unrestricted);
           let q = (if quant = KEYWORD KW_FORALL then Quant_Forall else Quant_Exists);
           return (\<lambda>loc. BabTm_Quantifier loc q (fst name_ty) (snd name_ty) tm)
+        })
+    <|> (do {
+          ty \<leftarrow> parse_numeric_type;
+          operand \<leftarrow> parens (delay (\<lambda>_. parse_term_min fuel 0 Unrestricted));
+          return (\<lambda>loc. BabTm_Cast loc ty operand)
+        })
+    <|> (do { 
+          expect (KEYWORD KW_CAST);
+          ty \<leftarrow> angles (delay (\<lambda>_. parse_type_fuelled fuel));
+          operand \<leftarrow> parens (delay (\<lambda>_. parse_term_min fuel 0 Unrestricted));
+          return (\<lambda>loc. BabTm_Cast loc ty operand)
+        })
+    <|> (do {
+          expect (KEYWORD KW_SIZEOF);
+          operand \<leftarrow> parens (delay (\<lambda>_. parse_term_min fuel 0 Unrestricted));
+          return (\<lambda>loc. BabTm_Sizeof loc operand)
+        })
+    <|> (do {
+          expect (KEYWORD KW_ALLOCATED);
+          operand \<leftarrow> parens (delay (\<lambda>_. parse_term_min fuel 0 Unrestricted));
+          return (\<lambda>loc. BabTm_Allocated loc operand)
+        })
+    <|> (do {
+          expect (KEYWORD KW_OLD);
+          operand \<leftarrow> parens (delay (\<lambda>_. parse_term_min fuel 0 Unrestricted));
+          return (\<lambda>loc. BabTm_Old loc operand)
+        })
+    <|> (do {
+          expect (KEYWORD KW_RETURN);
+          return (\<lambda>loc. BabTm_Name loc ''return'' [])
+        })
+    <|> (do {
+          terms \<leftarrow> brackets (comma_list (delay (\<lambda>_. parse_term_min fuel 0 Unrestricted)));
+          return (\<lambda>loc. BabTm_Literal loc (BabLit_Array terms))
+        })
+    <|> (do {
+          terms \<leftarrow> braces (comma_list (delay (\<lambda>_. parse_term_min fuel 0 Unrestricted)));
+          return (\<lambda>loc. BabTm_Tuple loc terms)
+        })
+    <|> braces (do {
+          baseTermOption \<leftarrow> optional (do {
+            term \<leftarrow> parse_term_min fuel 0 Unrestricted;
+            expect (KEYWORD KW_WITH);
+            return term });
+          namesTerms \<leftarrow> comma_list (delay (\<lambda>_. 
+            (do {
+              name \<leftarrow> parse_name;
+              expect EQUAL;
+              value \<leftarrow> parse_term_min fuel 0 Unrestricted;
+              return (name, value)
+            })));
+          return (\<lambda>loc. case baseTermOption of
+            None \<Rightarrow> BabTm_Record loc namesTerms
+            | Some baseTerm \<Rightarrow> BabTm_RecordUpdate loc baseTerm namesTerms)
         })
    )"
 
@@ -384,15 +453,694 @@ definition parse_type :: "BabType Parser" where
 definition parse_term :: "BabTerm Parser" where
   "parse_term = do {
     count \<leftarrow> get_num_tokens;
-    parse_term_min (Suc count) 0
+    parse_term_min (Suc count) 0 Unrestricted
+  }"
+
+definition parse_restricted_term :: "BabTerm Parser" where
+  "parse_restricted_term = do {
+    count \<leftarrow> get_num_tokens;
+    parse_term_min (Suc count) 0 Restricted
   }"
 
 
-(* Run a particular parser *)
+
+(* ATTRIBUTE PARSING *)
+
+definition parse_attribute :: "BabAttribute Parser" where
+  "parse_attribute = with_loc (do {
+    attrib \<leftarrow> 
+      (expect (KEYWORD KW_REQUIRES) \<then> return BabAttr_Requires)
+       <|> (expect (KEYWORD KW_ENSURES) \<then> return BabAttr_Ensures)
+       <|> (expect (KEYWORD KW_INVARIANT) \<then> return BabAttr_Invariant)
+       <|> (expect (KEYWORD KW_DECREASES) \<then> return BabAttr_Decreases);
+    term \<leftarrow> parse_term;
+    expect SEMICOLON;
+    return (\<lambda>loc. attrib loc term)
+  })"
+
+
+
+(* STATEMENT PARSING *)
+
+definition parse_var_decl_stmt :: "BabStatement Parser" where
+  "parse_var_decl_stmt = with_loc (do {
+    varOrRef \<leftarrow> (expect (KEYWORD KW_REF) \<then> return Ref)
+                <|> (expect (KEYWORD KW_VAR) \<then> return Var);
+    name \<leftarrow> parse_name;
+    maybeType \<leftarrow> optional (do {
+      expect COLON;
+      parse_type
+    });
+    maybeRhs \<leftarrow> (do {
+      expect EQUAL;
+      tm \<leftarrow> parse_term;
+      return (Some tm)
+    }) <|> (if varOrRef = Ref then fail else return None);
+    expect SEMICOLON;
+    return (\<lambda>loc. BabStmt_VarDecl loc name varOrRef maybeType maybeRhs)
+  })"
+
+definition parse_fix_stmt :: "BabStatement Parser" where
+  "parse_fix_stmt = with_loc (do {
+    expect (KEYWORD KW_FIX);
+    name \<leftarrow> parse_name;
+    expect COLON;
+    ty \<leftarrow> parse_type;
+    expect SEMICOLON;
+    return (\<lambda>loc. BabStmt_Fix loc name ty)
+  })"
+
+definition parse_obtain_stmt :: "BabStatement Parser" where
+  "parse_obtain_stmt = with_loc (do {
+    expect (KEYWORD KW_OBTAIN);
+    expect LPAREN;
+    name \<leftarrow> parse_name;
+    expect COLON;
+    ty \<leftarrow> parse_type;
+    expect RPAREN;
+    cond \<leftarrow> parse_term;
+    expect SEMICOLON;
+    return (\<lambda>loc. BabStmt_Obtain loc name ty cond)
+  })"
+
+definition parse_use_stmt :: "BabStatement Parser" where
+  "parse_use_stmt = with_loc (do {
+    expect (KEYWORD KW_USE);
+    tm \<leftarrow> parse_term;
+    expect SEMICOLON;
+    return (\<lambda>loc. BabStmt_Use loc tm)
+  })"
+
+definition parse_swap_stmt :: "BabStatement Parser" where
+  "parse_swap_stmt = with_loc (do {
+    expect (KEYWORD KW_SWAP);
+    lhs \<leftarrow> parse_term;
+    expect COMMA;
+    rhs \<leftarrow> parse_term;
+    expect SEMICOLON;
+    return (\<lambda>loc. BabStmt_Swap loc lhs rhs)
+  })"
+
+definition parse_return_stmt :: "BabStatement Parser" where
+  "parse_return_stmt = with_loc (do {
+    expect (KEYWORD KW_RETURN);
+    maybeTerm \<leftarrow> optional parse_term;
+    expect SEMICOLON;
+    return (\<lambda>loc. BabStmt_Return loc maybeTerm)
+  })"
+
+(* both of these begin with a term (as opposed to a keyword) *)
+definition parse_assignment_or_call_stmt :: "BabStatement Parser" where
+  "parse_assignment_or_call_stmt = with_loc (do {
+    lhs \<leftarrow> parse_term;
+    result \<leftarrow> (do {
+      expect EQUAL;
+      rhs \<leftarrow> parse_term;
+      return (\<lambda>loc. BabStmt_Assign loc lhs rhs)
+    }) <|> 
+      (case lhs of
+        BabTm_Call _ _ _ \<Rightarrow> return (\<lambda>loc. BabStmt_Call loc lhs)
+        | _ \<Rightarrow> fail);
+    expect SEMICOLON;
+    return result
+  })"
+
+definition parse_assume_stmt :: "BabStatement Parser" where
+  "parse_assume_stmt = with_loc (do {
+    cond \<leftarrow> parse_term;
+    return (\<lambda>loc. BabStmt_Assume loc cond)
+  })"
+
+definition parse_show_hide_stmt :: "BabStatement Parser" where
+  "parse_show_hide_stmt = with_loc (do {
+    showOrHide \<leftarrow> 
+      (expect (KEYWORD KW_SHOW) \<then> return Show)
+      <|> (expect (KEYWORD KW_HIDE) \<then> return Hide);
+    name \<leftarrow> parse_dotted_name;
+    expect SEMICOLON;
+    return (\<lambda>loc. BabStmt_ShowHide loc showOrHide name)
+  })"
+
+fun parse_assert_stmt :: "nat \<Rightarrow> BabStatement Parser"
+  and parse_if_stmt :: "nat \<Rightarrow> BabStatement Parser"
+  and parse_while_stmt :: "nat \<Rightarrow> BabStatement Parser"
+  and parse_stmt_fuelled :: "nat \<Rightarrow> BabStatement Parser"
+where
+  "parse_assert_stmt fuel = with_loc (do {
+    expect (KEYWORD KW_ASSERT);
+    maybeCond \<leftarrow> 
+      (parse_restricted_term \<bind> return \<circ> Some) 
+      <|> (expect STAR \<then> return None);
+    proof \<leftarrow> 
+      braces (many (delay (\<lambda>_. parse_stmt_fuelled fuel)))
+      <|> (expect SEMICOLON \<then> return []);
+    return (\<lambda>loc. BabStmt_Assert loc maybeCond proof)
+  })"
+
+| "parse_if_stmt fuel = with_loc (do {
+    expect (KEYWORD KW_IF);
+    cond \<leftarrow> parse_restricted_term;
+    thenBlock \<leftarrow> braces (many (delay (\<lambda>_. parse_stmt_fuelled fuel)));
+    elseBlock \<leftarrow>
+      (do {
+        expect (KEYWORD KW_ELSE);
+        braces (many (delay (\<lambda>_. parse_stmt_fuelled fuel))) 
+      })
+      <|> (do {
+        expect (KEYWORD KW_ELSE);
+        look_ahead (expect (KEYWORD KW_IF));
+        ifStmt \<leftarrow> parse_stmt_fuelled fuel;
+        return [ifStmt]
+      })
+      <|> (return []);
+    return (\<lambda>loc. BabStmt_If loc cond thenBlock elseBlock)
+  })"
+
+| "parse_while_stmt fuel = with_loc (do {
+    cond \<leftarrow> parse_restricted_term;
+    attrs \<leftarrow> many parse_attribute;
+    body \<leftarrow> many (delay (\<lambda>_. parse_stmt_fuelled fuel));
+    return (\<lambda>loc. BabStmt_While loc cond attrs body)
+  })"
+
+| "parse_stmt_fuelled 0 = undefined"   (* out of fuel *)
+| "parse_stmt_fuelled (Suc fuel) = 
+    parse_var_decl_stmt
+    <|> parse_fix_stmt
+    <|> parse_obtain_stmt
+    <|> parse_use_stmt
+    <|> parse_swap_stmt
+    <|> parse_return_stmt
+    <|> parse_assignment_or_call_stmt
+    <|> parse_assume_stmt
+    <|> parse_show_hide_stmt
+    <|> parse_assert_stmt fuel
+    <|> parse_if_stmt fuel
+    <|> parse_while_stmt fuel"
+
+
+(* Top-level statement parser *)
+definition parse_statement :: "BabStatement Parser" where
+  "parse_statement = do {
+    count \<leftarrow> get_num_tokens;
+    parse_stmt_fuelled (Suc count)
+  }"
+
+
+(* DECLARATION PARSING *)
+
+datatype EIG = Extern | Impure | Ghost
+
+definition parse_const_decl :: "BabDeclaration Parser" where
+  "parse_const_decl = with_loc (do {
+    ghost \<leftarrow> (do {
+      ghosts \<leftarrow> many (expect (KEYWORD KW_GHOST));
+      return (ghosts \<noteq> [])
+    });
+    expect (KEYWORD KW_CONST);
+    name \<leftarrow> parse_name;
+    type \<leftarrow> optional (expect COLON \<then> parse_type);
+    rhs \<leftarrow> optional (expect EQUAL \<then> parse_term);
+    expect SEMICOLON;
+    return (\<lambda>loc. BabDecl_Const \<lparr> DC_Location = loc,
+                                  DC_Name = name,
+                                  DC_Type = type,
+                                  DC_Value = rhs,
+                                  DC_Ghost = ghost \<rparr>)
+  })"
+
+definition parse_fun_arg :: "(string \<times> VarOrRef \<times> BabType) Parser" where
+  "parse_fun_arg = do {
+    ref0 \<leftarrow> optional (expect (KEYWORD KW_REF));
+    name \<leftarrow> parse_name;
+    expect COLON;
+    ref \<leftarrow> (if ref0 = None then optional (expect (KEYWORD KW_REF)) else return ref0);
+    type \<leftarrow> parse_type;
+    return (name, if ref = None then Var else Ref, type)
+  }"
+
+definition parse_function_decl :: "BabDeclaration Parser" where
+  "parse_function_decl = with_loc (do {
+    markers \<leftarrow> many
+      ((expect (KEYWORD KW_GHOST) \<then> return Ghost)
+       <|> (expect (KEYWORD KW_EXTERN) \<then> return Extern)
+       <|> (expect (KEYWORD KW_IMPURE) \<then> return Impure));
+    let markerSet = set markers;
+    expect (KEYWORD KW_FUNCTION);
+    name \<leftarrow> parse_name;
+    tyvars \<leftarrow> (angles (comma_list parse_name)) <|> (return []);
+    args \<leftarrow> parens (comma_list parse_fun_arg);
+    retType \<leftarrow> optional (expect COLON \<then> parse_type);
+    externName \<leftarrow> (if Extern \<in> markerSet then
+      (optional (do {
+        expect EQUAL;
+        t \<leftarrow> satisfy is_string_token;
+        case t of STRING s \<Rightarrow> return s }))
+      else return None);
+    optional (expect SEMICOLON);
+    attrs \<leftarrow> many parse_attribute;
+    body \<leftarrow> optional (braces (many parse_statement));
+    return (\<lambda>loc. BabDecl_Function \<lparr> DF_Location = loc,
+                                     DF_Name = name,
+                                     DF_TyArgs = tyvars,
+                                     DF_TmArgs = args,
+                                     DF_ReturnType = retType,
+                                     DF_Body = body,
+                                     DF_Attributes = attrs,
+                                     DF_Ghost = (Ghost \<in> markerSet),
+                                     DF_Extern = (Extern \<in> markerSet),
+                                     DF_Impure = (Impure \<in> markerSet) \<rparr>)
+  })"
+
+definition parse_data_ctor :: "DataCtor Parser" where
+  "parse_data_ctor = with_loc (do {
+    name \<leftarrow> parse_name;
+    payload \<leftarrow> optional (do {
+      look_ahead (expect LPAREN <|> expect LBRACE);
+      parse_type
+    });
+    return (\<lambda>loc. (loc, name, payload))
+  })"
+
+definition parse_datatype_decl :: "BabDeclaration Parser" where
+  "parse_datatype_decl = with_loc (do {
+    expect (KEYWORD KW_DATATYPE);
+    name \<leftarrow> parse_name;
+    tyvars \<leftarrow> (angles (comma_list parse_name)) <|> (return []);
+    expect EQUAL;
+    ctors \<leftarrow> sep_by_1 parse_data_ctor (expect BAR);
+    expect SEMICOLON;
+    return (\<lambda>loc. BabDecl_Datatype \<lparr> DD_Location = loc,
+                                     DD_Name = name,
+                                     DD_TyArgs = tyvars,
+                                     DD_Ctors = ctors \<rparr>)
+  })"
+
+definition parse_typedef_rhs :: "(BabType option \<times> AllocLevel) Parser" where
+  "parse_typedef_rhs = do {
+    expect EQUAL;
+    ty \<leftarrow> parse_type;
+    return (Some ty, AllocNever)
+  }"
+
+definition parse_typedef_alloc :: "(BabType option \<times> AllocLevel) Parser" where
+  "parse_typedef_alloc = parens (
+    (expect (KEYWORD KW_ALLOCATED) \<then> return (None, AllocIfNotDefault))
+    <|> (expect (NAME ''allocated_always'') \<then> return (None, AllocAlways))
+  )"
+
+definition parse_typedef_decl :: "BabDeclaration Parser" where
+  "parse_typedef_decl = with_loc (do {
+    extern \<leftarrow> (do {
+      externs \<leftarrow> many (expect (KEYWORD KW_EXTERN));
+      return (externs \<noteq> [])
+    });
+    expect (KEYWORD KW_TYPE);
+    name \<leftarrow> parse_name;
+    tyvars \<leftarrow> (angles (comma_list parse_name)) <|> (return []);
+    defnAlloc \<leftarrow> (if \<not>extern then parse_typedef_rhs else fail)
+      <|> (parse_typedef_alloc)
+      <|> (return (None, AllocNever));
+    expect SEMICOLON;
+    return (\<lambda>loc. BabDecl_Typedef \<lparr> DT_Location = loc,
+                                    DT_Name = name,
+                                    DT_TyArgs = tyvars,
+                                    DT_Definition = fst defnAlloc,
+                                    DT_Extern = extern,
+                                    DT_AllocLevel = snd defnAlloc \<rparr>)
+  })"
+
+definition parse_decl :: "BabDeclaration Parser" where
+  "parse_decl = parse_const_decl 
+    <|> parse_function_decl 
+    <|> parse_datatype_decl
+    <|> parse_typedef_decl"
+
+
+(* MODULE PARSING *)
+
+definition parse_import :: "BabImport Parser" where
+  "parse_import = with_loc (do {
+    expect (KEYWORD KW_IMPORT);
+    qualified \<leftarrow> (expect (NAME ''qualified'') \<then> return True) <|> (return False);
+    name \<leftarrow> parse_dotted_name;
+    alias \<leftarrow> (expect (NAME ''as'') \<then> parse_name) <|> (return name);
+    expect SEMICOLON;
+    return (\<lambda>loc. \<lparr> Imp_Location = loc,
+                    Imp_ModuleName = name,
+                    Imp_AliasName = alias,
+                    Imp_Qualified = qualified \<rparr>)
+  })"
+
+(* this parses a complete module including the following eof *)
+definition parse_module :: "BabModule Parser" where
+  "parse_module = do {
+    expect (KEYWORD KW_MODULE);
+    name \<leftarrow> parse_dotted_name;
+    interface_imports \<leftarrow> many parse_import;
+    expect (KEYWORD KW_INTERFACE);
+    interface \<leftarrow> braces (many parse_decl);
+    impl_imports \<leftarrow> many parse_import;
+    impl \<leftarrow> many parse_decl;
+    eof;
+    return \<lparr> Mod_Name = name,
+             Mod_InterfaceImports = interface_imports,
+             Mod_Interface = interface,
+             Mod_ImplementationImports = impl_imports,
+             Mod_Implementation = impl \<rparr>
+  }"
+
+
+(* FUNCTION TO RUN A PARSER *)
+
 definition run_parser :: "'a Parser \<Rightarrow> string \<Rightarrow> (Location \<times> Token) list \<Rightarrow> 'a ParseResult" where
   "run_parser parser filename lexerResult =
     (let initialState = initial_parser_state filename lexerResult in
      parser initialState)"
+
+
+(* POST-PARSING CHECKS *)
+
+datatype PostParseError = 
+  PPE_MixedArrayDimension
+  | PPE_OldOutsidePostcondition
+  | PPE_ReturnOutsidePostcondition
+  | PPE_DataCtorWrongCase
+
+fun array_dims_valid :: "BabDimension list \<Rightarrow> bool" where
+  "array_dims_valid [] = True"
+| "array_dims_valid (BabDim_Unknown # dims) = list_all (\<lambda>x. x = BabDim_Unknown) dims"
+| "array_dims_valid (BabDim_Allocatable # dims) = list_all (\<lambda>x. x = BabDim_Allocatable) dims"
+| "array_dims_valid (BabDim_Fixed _ # dims) = list_all (\<lambda>x. case x of
+                                                 BabDim_Fixed _ \<Rightarrow> True
+                                                 | _ \<Rightarrow> False) dims"
+
+definition ttsize :: "BabType + BabTerm \<Rightarrow> nat"
+  where "ttsize = case_sum bab_type_size bab_term_size"
+
+(* note: these functions return PPE_OldOutsidePostcondition and/or 
+   PPE_ReturnOutsidePostcondition if applicable. These must be filtered out
+   afterwards if the term actually is part of a postcondition. *)
+function post_parse_type :: "BabType \<Rightarrow> (Location \<times> PostParseError) list"
+  and post_parse_term :: "BabTerm \<Rightarrow> (Location \<times> PostParseError) list"
+where
+  "post_parse_type (BabTy_Name _ _ types) = concat (map post_parse_type types)"
+| "post_parse_type (BabTy_Bool _) = []"
+| "post_parse_type (BabTy_FiniteInt _ _ _) = []"
+| "post_parse_type (BabTy_MathInt _) = []"
+| "post_parse_type (BabTy_MathReal _) = []"
+| "post_parse_type (BabTy_Tuple _ types) = concat (map post_parse_type types)"
+| "post_parse_type (BabTy_Record _ fieldTypes) = concat (map (post_parse_type \<circ> snd) fieldTypes)"
+| "post_parse_type (BabTy_Array loc eltType dims) =
+    post_parse_type eltType
+    @ (if array_dims_valid dims then [] else [(loc, PPE_MixedArrayDimension)])
+    @ (concat (map post_parse_term (concat (map array_dim_terms dims))))"
+
+| "post_parse_term (BabTm_Literal _ lit) = 
+    (case lit of
+      BabLit_Array tms \<Rightarrow> concat (map post_parse_term tms)
+      | _ \<Rightarrow> [])"
+| "post_parse_term (BabTm_Name loc name types) = 
+     (if name = ''return'' then [(loc, PPE_ReturnOutsidePostcondition)] else [])
+     @ concat (map post_parse_type types)"
+| "post_parse_term (BabTm_Cast _ ty tm) = post_parse_type ty @ post_parse_term tm"
+| "post_parse_term (BabTm_If _ tm1 tm2 tm3) = 
+    post_parse_term tm1 @ post_parse_term tm2 @ post_parse_term tm3"
+| "post_parse_term (BabTm_Unop _ _ tm) = post_parse_term tm"
+| "post_parse_term (BabTm_Binop _ tm lst) = post_parse_term tm
+      @ concat (map (post_parse_term \<circ> snd) lst)"
+| "post_parse_term (BabTm_Let _ _ tm1 tm2) = post_parse_term tm1 @ post_parse_term tm2"
+| "post_parse_term (BabTm_Quantifier _ _ _ ty tm) = post_parse_type ty @ post_parse_term tm"
+| "post_parse_term (BabTm_Call _ tm tms) = post_parse_term tm @ concat (map post_parse_term tms)"
+| "post_parse_term (BabTm_Tuple _ tms) = concat (map post_parse_term tms)"
+| "post_parse_term (BabTm_Record _ flds) = concat (map (post_parse_term \<circ> snd) flds)"
+| "post_parse_term (BabTm_RecordUpdate _ tm flds) = post_parse_term tm
+      @ concat (map (post_parse_term \<circ> snd) flds)"
+| "post_parse_term (BabTm_TupleProj _ tm _) = post_parse_term tm"
+| "post_parse_term (BabTm_RecordProj _ tm _) = post_parse_term tm"
+| "post_parse_term (BabTm_ArrayProj _ tm tms) = post_parse_term tm 
+      @ concat (map post_parse_term tms)"
+| "post_parse_term (BabTm_Sizeof _ tm) = post_parse_term tm"
+| "post_parse_term (BabTm_Allocated _ tm) = post_parse_term tm"
+| "post_parse_term (BabTm_Old loc tm) = (loc, PPE_OldOutsidePostcondition) # post_parse_term tm"
+
+  by pat_completeness auto
+
+termination
+proof (relation "measure ttsize")
+  show "wf (measure ttsize)" by auto
+
+next
+  fix x loc name types
+  show "x \<in> set types \<Longrightarrow>
+       (Inl x, Inl (BabTy_Name loc name types)) \<in> measure ttsize"
+    unfolding ttsize_def using bab_type_smaller_than_list
+    by auto
+
+next
+  fix loc types x
+  show "x \<in> set types \<Longrightarrow>
+       (Inl x, Inl (BabTy_Tuple loc types)) \<in> measure ttsize"
+    unfolding ttsize_def using bab_type_smaller_than_list by auto
+
+next
+  fix loc fieldTypes x
+  show "x \<in> set fieldTypes \<Longrightarrow>
+       (Inl (snd x), Inl (BabTy_Record loc fieldTypes)) \<in> measure ttsize"
+    unfolding ttsize_def using bab_type_smaller_than_fieldlist
+    by (metis bab_type_size.simps(7) eq_snd_iff in_measure old.sum.simps(5)
+        plus_1_eq_Suc) 
+
+next
+  fix loc eltType dims
+  show "(Inl eltType, Inl (BabTy_Array loc eltType dims)) \<in> measure ttsize"
+    unfolding ttsize_def by auto
+
+next
+  fix loc eltType dims x
+  show "x \<in> set (concat (map array_dim_terms dims)) \<Longrightarrow>
+       (Inr x, Inl (BabTy_Array loc eltType dims)) \<in> measure ttsize"
+    unfolding ttsize_def using bab_term_smaller_than_arraydim by force
+
+next
+  fix loc lit tms tm
+  show "lit = BabLit_Array tms \<Longrightarrow>
+       tm \<in> set tms \<Longrightarrow> 
+       (Inr tm, Inr (BabTm_Literal loc lit)) \<in> measure ttsize"
+    unfolding ttsize_def using bab_term_smaller_than_list by force
+
+next
+  fix ty types loc name
+  show "ty \<in> set types \<Longrightarrow> (Inl ty, Inr (BabTm_Name loc name types)) \<in> measure ttsize"
+    unfolding ttsize_def using bab_type_smaller_than_list by force
+
+next
+  fix loc ty tm
+  show "(Inl ty, Inr (BabTm_Cast loc ty tm)) \<in> measure ttsize"
+    unfolding ttsize_def by auto
+
+next
+  fix loc ty tm
+  show "(Inr tm, Inr (BabTm_Cast loc ty tm)) \<in> measure ttsize"
+    unfolding ttsize_def by auto
+
+next
+  fix loc tm1 tm2 tm3
+  show "(Inr tm1, Inr (BabTm_If loc tm1 tm2 tm3)) \<in> measure ttsize"
+    unfolding ttsize_def by auto
+
+next
+  fix loc tm1 tm2 tm3
+  show "(Inr tm2, Inr (BabTm_If loc tm1 tm2 tm3)) \<in> measure ttsize"
+    unfolding ttsize_def by auto
+
+next
+  fix loc tm1 tm2 tm3
+  show "(Inr tm3, Inr (BabTm_If loc tm1 tm2 tm3)) \<in> measure ttsize"
+    unfolding ttsize_def by auto
+
+next
+  fix loc op tm
+  show "(Inr tm, Inr (BabTm_Unop loc op tm)) \<in> measure ttsize"
+    unfolding ttsize_def by auto
+
+next
+  fix loc tm lst
+  show "(Inr tm, Inr (BabTm_Binop loc tm lst)) \<in> measure ttsize"
+    unfolding ttsize_def by auto
+
+next
+  fix loc tm
+  fix lst :: "(BabBinop \<times> BabTerm) list"
+  fix x :: "BabBinop \<times> BabTerm"
+  assume Elem: "x \<in> set lst"
+  show "(Inr (snd x), Inr (BabTm_Binop loc tm lst)) \<in> measure ttsize"
+  proof (cases x)
+    case (Pair op rhs)
+    have "bab_term_size rhs < Suc (sum_list (map (bab_term_size \<circ> snd) lst))"
+      unfolding ttsize_def using bab_term_smaller_than_fieldlist Pair Elem by auto
+    thus ?thesis
+      by (simp add: Pair ttsize_def)
+  qed
+
+next
+  fix loc name tm1 tm2
+  show "(Inr tm1, Inr (BabTm_Let loc name tm1 tm2)) \<in> measure ttsize"
+    unfolding ttsize_def by auto
+
+next
+  fix loc name tm1 tm2
+  show "(Inr tm2, Inr (BabTm_Let loc name tm1 tm2)) \<in> measure ttsize"
+    unfolding ttsize_def by auto
+
+next
+  fix loc quant name ty tm
+  show "(Inl ty, Inr (BabTm_Quantifier loc quant name ty tm)) \<in> measure ttsize"
+    unfolding ttsize_def by auto
+
+next
+  fix loc quant name ty tm
+  show "(Inr tm, Inr (BabTm_Quantifier loc quant name ty tm)) \<in> measure ttsize"
+    unfolding ttsize_def by auto
+
+next
+  fix loc tm tms
+  show "(Inr tm, Inr (BabTm_Call loc tm tms)) \<in> measure ttsize"
+    unfolding ttsize_def by auto
+
+next
+  fix loc tm tms x
+  show "x \<in> set tms \<Longrightarrow> (Inr x, Inr (BabTm_Call loc tm tms)) \<in> measure ttsize"
+    unfolding ttsize_def using bab_term_smaller_than_list by force
+
+next
+  fix loc tms x
+  show "x \<in> set tms \<Longrightarrow> (Inr x, Inr (BabTm_Tuple loc tms)) \<in> measure ttsize"
+    unfolding ttsize_def using bab_term_smaller_than_list by force
+
+next
+  fix loc flds x
+  show "x \<in> set flds \<Longrightarrow> (Inr (snd x), Inr (BabTm_Record loc flds)) \<in> measure ttsize"
+    unfolding ttsize_def using bab_term_smaller_than_fieldlist
+    by (metis bab_term_size.simps(11) in_measure old.sum.simps(6) plus_1_eq_Suc
+        prod.exhaust_sel)
+
+next
+  fix loc tm flds 
+  show "(Inr tm, Inr (BabTm_RecordUpdate loc tm flds)) \<in> measure ttsize"
+    unfolding ttsize_def using bab_term_smaller_than_fieldlist by force
+
+next
+  fix loc tm flds x
+  show "x \<in> set flds \<Longrightarrow> (Inr (snd x), Inr (BabTm_RecordUpdate loc tm flds)) \<in> measure ttsize"
+    unfolding ttsize_def using bab_term_smaller_than_fieldlist
+    by (metis add_Suc_shift bab_term_size.simps(12) in_measure old.sum.simps(6) plus_1_eq_Suc
+        surjective_pairing trans_less_add2) 
+
+next
+  fix loc tm idx
+  show "(Inr tm, Inr (BabTm_TupleProj loc tm idx)) \<in> measure ttsize"
+    unfolding ttsize_def by auto
+
+next
+  fix loc tm name
+  show "(Inr tm, Inr (BabTm_RecordProj loc tm name)) \<in> measure ttsize"
+    unfolding ttsize_def by auto
+
+next
+  fix loc tm tms
+  show "(Inr tm, Inr (BabTm_ArrayProj loc tm tms)) \<in> measure ttsize"
+    unfolding ttsize_def by auto
+
+next
+  fix loc tm tms x
+  show "x \<in> set tms \<Longrightarrow> (Inr x, Inr (BabTm_ArrayProj loc tm tms)) \<in> measure ttsize"
+    unfolding ttsize_def using bab_term_smaller_than_list by force
+
+next
+  fix loc tm
+  show "(Inr tm, Inr (BabTm_Sizeof loc tm)) \<in> measure ttsize"
+    unfolding ttsize_def by auto
+
+next
+  fix loc tm
+  show "(Inr tm, Inr (BabTm_Allocated loc tm)) \<in> measure ttsize"
+    unfolding ttsize_def by auto
+
+next
+  fix loc tm
+  show "(Inr tm, Inr (BabTm_Old loc tm)) \<in> measure ttsize"
+    unfolding ttsize_def by auto
+
+qed
+
+
+fun post_parse_attribute :: "BabAttribute \<Rightarrow> (Location \<times> PostParseError) list" where
+  "post_parse_attribute (BabAttr_Requires _ tm) = post_parse_term tm"
+| "post_parse_attribute (BabAttr_Ensures _ tm) = 
+    filter (\<lambda>(_, err). err \<notin> {PPE_ReturnOutsidePostcondition, PPE_OldOutsidePostcondition})
+      (post_parse_term tm)"
+| "post_parse_attribute (BabAttr_Invariant _ tm) = post_parse_term tm"
+| "post_parse_attribute (BabAttr_Decreases _ tm) = post_parse_term tm"
+
+
+fun post_parse_statement :: "BabStatement \<Rightarrow> (Location \<times> PostParseError) list" where
+  "post_parse_statement (BabStmt_VarDecl _ _ _ maybeType maybeTerm) =
+    case_option [] post_parse_type maybeType 
+    @ case_option [] post_parse_term maybeTerm"
+| "post_parse_statement (BabStmt_Fix _ _ ty) = post_parse_type ty"
+| "post_parse_statement (BabStmt_Obtain _ _ ty tm) = post_parse_type ty @ post_parse_term tm"
+| "post_parse_statement (BabStmt_Use _ tm) = post_parse_term tm"
+| "post_parse_statement (BabStmt_Assign _ tm1 tm2) = post_parse_term tm1 @ post_parse_term tm2"
+| "post_parse_statement (BabStmt_Swap _ tm1 tm2) = post_parse_term tm1 @ post_parse_term tm2"
+| "post_parse_statement (BabStmt_Return _ maybeTm) = case_option [] post_parse_term maybeTm"
+| "post_parse_statement (BabStmt_Assert _ maybeTm stmts) =
+    case_option [] post_parse_term maybeTm
+    @ concat (map post_parse_statement stmts)"
+| "post_parse_statement (BabStmt_Assume _ tm) = post_parse_term tm"
+| "post_parse_statement (BabStmt_If _ tm stmts1 stmts2) =
+    post_parse_term tm
+    @ concat (map post_parse_statement stmts1)
+    @ concat (map post_parse_statement stmts2)"
+| "post_parse_statement (BabStmt_While _ tm attrs stmts) =
+    post_parse_term tm
+    @ concat (map post_parse_attribute attrs)
+    @ concat (map post_parse_statement stmts)"
+| "post_parse_statement (BabStmt_Call _ tm) = post_parse_term tm"
+| "post_parse_statement (BabStmt_ShowHide _ _ _) = []"
+
+
+fun begins_with_capital :: "string \<Rightarrow> bool" where
+  "begins_with_capital [] = False"
+| "begins_with_capital (c # cs) = (CHR ''A'' \<le> c \<and> c \<le> CHR ''Z'')"
+
+
+fun post_parse_data_ctor :: "Location \<times> string \<times> (BabType option) 
+    \<Rightarrow> (Location \<times> PostParseError) list" where
+"post_parse_data_ctor (loc, name, maybeTy) =
+   (if begins_with_capital name then [] else [(loc, PPE_DataCtorWrongCase)])
+   @ case_option [] post_parse_type maybeTy"
+
+
+fun post_parse_declaration :: "BabDeclaration \<Rightarrow> (Location \<times> PostParseError) list" where
+  "post_parse_declaration (BabDecl_Const cst) =
+    case_option [] post_parse_type (DC_Type cst)
+    @ case_option [] post_parse_term (DC_Value cst)"
+| "post_parse_declaration (BabDecl_Function fun) =
+    concat (map (\<lambda>(_,_,ty). post_parse_type ty) (DF_TmArgs fun))
+    @ case_option [] post_parse_type (DF_ReturnType fun)
+    @ case_option [] (concat \<circ> map post_parse_statement) (DF_Body fun)
+    @ concat (map post_parse_attribute (DF_Attributes fun))"
+| "post_parse_declaration (BabDecl_Datatype dtype) =
+    concat (map post_parse_data_ctor (DD_Ctors dtype))"
+| "post_parse_declaration (BabDecl_Typedef tydef) =
+    case_option [] post_parse_type (DT_Definition tydef)"
+
+
+fun post_parse_module :: "BabModule \<Rightarrow> (Location \<times> PostParseError) list" where
+  "post_parse_module module =
+    concat (map post_parse_declaration (Mod_Interface module))
+    @ concat (map post_parse_declaration (Mod_Implementation module))"
 
 
 end
