isabelle/BabSyntax.thy
@@ -197,7 +197,7 @@ and BabTerm =
   | BabTm_Cast Location BabType BabTerm
   | BabTm_If Location BabTerm BabTerm BabTerm
   | BabTm_Unop Location BabUnop BabTerm
-  | BabTm_Binop Location BabBinop BabTerm BabTerm
+  | BabTm_Binop Location BabTerm "(BabBinop \<times> BabTerm) list"  (* all ops have same precedence *)
   | BabTm_Let Location string BabTerm BabTerm
   | BabTm_Quantifier Location Quantifier string BabType BabTerm
   | BabTm_Call Location BabTerm "BabTerm list"
@@ -207,12 +207,94 @@ and BabTerm =
   | BabTm_TupleProj Location BabTerm nat
   | BabTm_RecordProj Location BabTerm string
   | BabTm_ArrayProj Location BabTerm "BabTerm list"
-  (* omitted for now: BabTerm_Match *)
+  (* omitted for now: BabTm_Match *)
   | BabTm_Sizeof Location BabTerm
   | BabTm_Allocated Location BabTerm
+  | BabTm_Old Location BabTerm
+
+datatype BabAttribute = 
+  BabAttr_Requires Location BabTerm
+  | BabAttr_Ensures Location BabTerm
+  | BabAttr_Invariant Location BabTerm
+  | BabAttr_Decreases Location BabTerm
+
+datatype ShowOrHide = Show | Hide
+datatype VarOrRef = Var | Ref
+
+datatype BabStatement =
+  BabStmt_VarDecl Location string VarOrRef "BabType option" "BabTerm option"
+  | BabStmt_Fix Location string BabType
+  | BabStmt_Obtain Location string BabType BabTerm
+  | BabStmt_Use Location BabTerm
+  | BabStmt_Assign Location BabTerm BabTerm
+  | BabStmt_Swap Location BabTerm BabTerm
+  | BabStmt_Return Location "BabTerm option"
+  | BabStmt_Assert Location "BabTerm option" "BabStatement list"
+  | BabStmt_Assume Location BabTerm
+  | BabStmt_If Location BabTerm "BabStatement list" "BabStatement list"
+  | BabStmt_While Location BabTerm "BabAttribute list" "BabStatement list"
+  | BabStmt_Call Location BabTerm   (* BabTm_Call term *)
+  | BabStmt_ShowHide Location ShowOrHide string
+
+datatype AllocLevel = AllocNever | AllocIfNotDefault | AllocAlways
+
+record DeclConst =
+  DC_Location :: Location
+  DC_Name :: string
+  DC_Type :: "BabType option"
+  DC_Value :: "BabTerm option"
+  DC_Ghost :: bool
+
+record DeclFun =
+  DF_Location :: Location
+  DF_Name :: string
+  DF_TyArgs :: "string list"
+  DF_TmArgs :: "(string \<times> VarOrRef \<times> BabType) list"
+  DF_ReturnType :: "BabType option"
+  DF_Body :: "(BabStatement list) option"
+  DF_Attributes :: "BabAttribute list"
+  DF_Ghost :: bool
+  DF_Extern :: bool
+  DF_Impure :: bool
+
+type_synonym DataCtor = "Location \<times> string \<times> (BabType option)"
+
+record DeclDatatype =
+  DD_Location :: Location
+  DD_Name :: string
+  DD_TyArgs :: "string list"
+  DD_Ctors :: "DataCtor list"
+
+record DeclTypedef = 
+  DT_Location :: Location
+  DT_Name :: string
+  DT_TyArgs :: "string list"
+  DT_Definition :: "BabType option"   (* `None` for abstract or extern type *)
+  DT_Extern :: bool
+  DT_AllocLevel :: AllocLevel   (* Only relevant if DT_Definition is None *)
+
+datatype BabDeclaration = 
+  BabDecl_Const DeclConst
+  | BabDecl_Function DeclFun
+  | BabDecl_Datatype DeclDatatype
+  | BabDecl_Typedef DeclTypedef
+
+record BabImport =
+  Imp_Location :: Location
+  Imp_ModuleName :: string
+  Imp_AliasName :: string
+  Imp_Qualified :: bool
+
+record BabModule =
+  Mod_Name :: string
+  Mod_InterfaceImports :: "BabImport list"
+  Mod_Interface :: "BabDeclaration list"
+  Mod_ImplementationImports :: "BabImport list"
+  Mod_Implementation :: "BabDeclaration list"
 
 
-(* Helper functions for the abstract syntax *)
+
+(* Helper functions *)
 
 fun bab_type_location :: "BabType \<Rightarrow> Location" where
   "bab_type_location (BabTy_Name loc _ _) = loc"
@@ -230,7 +312,7 @@ fun bab_term_location :: "BabTerm \<Rightarrow> Location" where
 | "bab_term_location (BabTm_Cast loc _ _) = loc"
 | "bab_term_location (BabTm_If loc _ _ _) = loc"
 | "bab_term_location (BabTm_Unop loc _ _) = loc"
-| "bab_term_location (BabTm_Binop loc _ _ _) = loc"
+| "bab_term_location (BabTm_Binop loc _ _) = loc"
 | "bab_term_location (BabTm_Let loc _ _ _) = loc"
 | "bab_term_location (BabTm_Quantifier loc _ _ _ _) = loc"
 | "bab_term_location (BabTm_Call loc _ _) = loc"
@@ -242,7 +324,119 @@ fun bab_term_location :: "BabTerm \<Rightarrow> Location" where
 | "bab_term_location (BabTm_ArrayProj loc _ _) = loc"
 | "bab_term_location (BabTm_Sizeof loc _) = loc"
 | "bab_term_location (BabTm_Allocated loc _) = loc"
+| "bab_term_location (BabTm_Old loc _) = loc"
+
+fun bab_attribute_location :: "BabAttribute \<Rightarrow> Location" where
+  "bab_attribute_location (BabAttr_Requires loc _) = loc"
+| "bab_attribute_location (BabAttr_Ensures loc _) = loc"
+| "bab_attribute_location (BabAttr_Invariant loc _) = loc"
+| "bab_attribute_location (BabAttr_Decreases loc _) = loc"
+
+fun bab_statement_location :: "BabStatement \<Rightarrow> Location" where
+  "bab_statement_location (BabStmt_VarDecl loc _ _ _ _) = loc"
+| "bab_statement_location (BabStmt_Fix loc _ _) = loc"
+| "bab_statement_location (BabStmt_Obtain loc _ _ _) = loc"
+| "bab_statement_location (BabStmt_Use loc _) = loc"
+| "bab_statement_location (BabStmt_Assign loc _ _) = loc"
+| "bab_statement_location (BabStmt_Swap loc _ _) = loc"
+| "bab_statement_location (BabStmt_Return loc _) = loc"
+| "bab_statement_location (BabStmt_Assert loc _ _) = loc"
+| "bab_statement_location (BabStmt_Assume loc _) = loc"
+| "bab_statement_location (BabStmt_If loc _ _ _) = loc"
+| "bab_statement_location (BabStmt_While loc _ _ _) = loc"
+| "bab_statement_location (BabStmt_Call loc _) = loc"
+| "bab_statement_location (BabStmt_ShowHide loc _ _) = loc"
+
+fun array_dim_terms :: "BabDimension \<Rightarrow> BabTerm list" where
+  "array_dim_terms (BabDim_Fixed tm) = [tm]"
+| "array_dim_terms _ = []"
 
 
+
+(* Size functions *)
+
+fun bab_literal_size :: "BabLiteral \<Rightarrow> nat"
+  and bab_dimension_size :: "BabDimension \<Rightarrow> nat"
+  and bab_type_size :: "BabType \<Rightarrow> nat"
+  and bab_term_size :: "BabTerm \<Rightarrow> nat"
+where
+"bab_literal_size (BabLit_Array terms) = 1 + sum_list (map bab_term_size terms)"
+| "bab_literal_size _ = 1"
+| "bab_dimension_size (BabDim_Fixed tm) = 1 + bab_term_size tm"
+| "bab_dimension_size _ = 1"
+| "bab_type_size (BabTy_Name _ _ tyargs) = 1 + sum_list (map bab_type_size tyargs)"
+| "bab_type_size (BabTy_Bool _) = 1"
+| "bab_type_size (BabTy_FiniteInt _ _ _) = 1"
+| "bab_type_size (BabTy_MathInt _) = 1"
+| "bab_type_size (BabTy_MathReal _) = 1"
+| "bab_type_size (BabTy_Tuple _ types) = 1 + sum_list (map bab_type_size types)"
+| "bab_type_size (BabTy_Record _ flds) = 1 + sum_list (map (bab_type_size \<circ> snd) flds)"
+| "bab_type_size (BabTy_Array _ ty dims) = 1 + bab_type_size ty + sum_list (map bab_dimension_size dims)"
+| "bab_term_size (BabTm_Literal _ lit) = 1 + bab_literal_size lit"
+| "bab_term_size (BabTm_Name _ _ types) = 1 + sum_list (map bab_type_size types)"
+| "bab_term_size (BabTm_Cast _ ty tm) = 1 + bab_type_size ty + bab_term_size tm"
+| "bab_term_size (BabTm_If _ tm1 tm2 tm3) = 
+    1 + bab_term_size tm1 + bab_term_size tm2 + bab_term_size tm3"
+| "bab_term_size (BabTm_Unop _ _ tm) = 1 + bab_term_size tm"
+| "bab_term_size (BabTm_Binop _ tm items) = 
+    1 + bab_term_size tm + sum_list (map (bab_term_size \<circ> snd) items)"
+| "bab_term_size (BabTm_Let _ _ tm1 tm2) = 1 + bab_term_size tm1 + bab_term_size tm2"
+| "bab_term_size (BabTm_Quantifier _ _ _ ty tm) = 1 + bab_type_size ty + bab_term_size tm"
+| "bab_term_size (BabTm_Call _ tm args) = 1 + bab_term_size tm + sum_list (map bab_term_size args)"
+| "bab_term_size (BabTm_Tuple _ terms) = 1 + sum_list (map bab_term_size terms)"
+| "bab_term_size (BabTm_Record _ flds) = 1 + sum_list (map (bab_term_size \<circ> snd) flds)"
+| "bab_term_size (BabTm_RecordUpdate _ tm flds) = 
+    1 + bab_term_size tm + sum_list (map (bab_term_size \<circ> snd) flds)"
+| "bab_term_size (BabTm_TupleProj _ tm _) = 1 + bab_term_size tm"
+| "bab_term_size (BabTm_RecordProj _ tm _) = 1 + bab_term_size tm"
+| "bab_term_size (BabTm_ArrayProj _ tm indices) = 
+    1 + bab_term_size tm + sum_list (map bab_term_size indices)"
+| "bab_term_size (BabTm_Sizeof _ tm) = 1 + bab_term_size tm"
+| "bab_term_size (BabTm_Allocated _ tm) = 1 + bab_term_size tm"
+| "bab_term_size (BabTm_Old _ tm) = 1 + bab_term_size tm"
+
+
+lemma bab_type_smaller_than_list:
+  "ty \<in> set types \<Longrightarrow> bab_type_size ty < Suc (sum_list (map bab_type_size types))"
+  by (induction types, auto)
+
+lemma bab_type_smaller_than_fieldlist:
+  "(name, ty) \<in> set fieldTypes \<Longrightarrow> 
+    bab_type_size ty < Suc (sum_list (map (bab_type_size \<circ> snd) fieldTypes))"
+  by (induction fieldTypes, auto)
+
+lemma bab_term_smaller_than_list:
+  "tm \<in> set terms \<Longrightarrow> bab_term_size tm < Suc (sum_list (map bab_term_size terms))"
+  by (induction terms, auto)
+
+lemma bab_term_smaller_than_fieldlist:
+  "(name, tm) \<in> set flds \<Longrightarrow>
+    bab_term_size tm < Suc (sum_list (map (bab_term_size \<circ> snd) flds))"
+  by (induction flds, auto)
+
+lemma bab_term_smaller_than_arraydim:
+  assumes "dim \<in> set dims"
+    and "tm \<in> set (array_dim_terms dim)"
+  shows "bab_term_size tm < Suc (sum_list (map bab_dimension_size dims))"
+using assms
+proof (induction dims)
+  case Nil
+  then show ?case by auto
+next
+  case (Cons dim1 dimRest)
+  then show ?case proof (cases "dim = dim1")
+    case True
+    have "array_dim_terms dim = [tm]" using assms(2)
+      by (metis array_dim_terms.elims distinct.simps(2) distinct_singleton set_ConsD)
+    hence "bab_dimension_size dim1 = 1 + bab_term_size tm"
+      by (metis BabDimension.distinct(3,5) BabDimension.inject True array_dim_terms.elims
+          bab_dimension_size.elims list.distinct(1) list.inject)
+    thus ?thesis
+      by simp
+  next
+    case False
+    then show ?thesis using Cons by auto
+  qed
+qed
 
 end
